terms/cnterm.v
@@ -2,6 +2,8 @@
 
   Copyright 2014 Cornell University
   Copyright 2015 Cornell University
+  Copyright 2016 Cornell University
+  Copyright 2017 Cornell University
 
   This file is part of VPrl (the Verified Nuprl project).
 
@@ -19,7 +21,10 @@
   along with VPrl.  If not, see <http://www.gnu.org/licenses/>.
 
 
-  Website: http://nuprl.org/html/verification/
+  Websites: http://nuprl.org/html/verification/
+            http://nuprl.org/html/Nuprl2Coq
+            https://github.com/vrahli/NuprlInCoq
+
   Authors: Abhishek Anand & Vincent Rahli & Mark Bickford
 
 *)
@@ -222,6 +227,7 @@ Lemma lsubstc_mk_natk2nout_sp1 {o} :
       (lsubstc (mk_natk2nout (mk_var v)) w ((v,t) :: s) c)
       (natk2nout t).
 Proof.
+  Opaque beq_var.
   introv.
   unfold alphaeqc; simpl.
   unfold csubst.
